Fix generators etc.

library/modelled.v
@@ -5,89 +5,8 @@ Require Import Psatz.
 Require Import List.
 Import ListNotations.
 
-Class Isomorphism (A B : Type) :=
-  { from : A -> B
-  ; to : B -> A
-  ; from_to : forall (x : A), to (from x) = x
-  ; to_from : forall (x : B), from (to x) = x
-  }.
-
-Instance Isomorphism_refl {A : Type} : Isomorphism A A.
-Proof.
-  refine {| from := id ; to := id ; from_to := _ ; to_from := _ |}; auto.
-Defined.
-
-Lemma Isomorphism_sym {A B : Type} : Isomorphism A B -> Isomorphism B A.
-Proof.
-  intro i.
-  exact {| from := to
-         ; to := from
-         ; from_to := to_from
-         ; to_from := from_to |}.
-Defined.
-
-Lemma Isomorphism_trans {A B C : Type} : Isomorphism A B -> Isomorphism B C -> Isomorphism A C.
-Proof.
-  intros [f1 t1 pf1 pt1] [f2 t2 pf2 pt2].
-  refine {| from := fun x => f2 (f1 x)
-          ; to := fun x => t1 (t2 x)
-          ; from_to := _
-          ; to_from := _ |};
-  intro; [rewrite pf2, pf1 | rewrite pt1, pt2]; auto.
-Defined.
-
-Lemma from_sym : forall A B `(M : Isomorphism A B),
-    @from A B M = @to B A (Isomorphism_sym M).
-Proof.
-  intros A B M; auto.
-Defined.
-
-Lemma to_sym : forall A B `(M : Isomorphism A B),
-    @to A B M = @from B A (Isomorphism_sym M).
-Proof.
-  intros A B M; auto.
-Defined.
-
-Lemma from_trans : forall A B C `(M1 : Isomorphism A B) `(M2 : Isomorphism B C),
-    forall (x : A), @from B C M2 (@from A B M1 x) = @from A C (Isomorphism_trans M1 M2) x .
-Proof.
-  intros A B C [f1 t1 pf1 pt1] [f2 t2 pf2 pt2] x; simpl; auto.
-Defined.
-
-
-Require Import Coq.Logic.FunctionalExtensionality.
-
-Lemma Isomorphism_dep_fn {A A' : Type} {B : A -> Type} {B' : A' -> Type} :
-  Isomorphism A A' ->
-  (forall (a : A) (a' : A'), Isomorphism A A' -> Isomorphism (B a) (B' a')) ->
-  Isomorphism (forall (a : A), B a) (forall (a' : A'), B' a').
-Proof.
-  intros.
-  econstructor.
-  instantiate (1 := ltac:(intros g a; exact (from (g (to a))))).
-  instantiate (1 := ltac:(intros g a'; exact (to (g (from a'))))).
-  all: intros; apply functional_extensionality_dep;
-       intro; rewrite ?from_to, ?to_from; auto.
-Defined.
-
-Lemma Isomorphism_fn {A A' B B' : Type} :
-  Isomorphism A A' -> Isomorphism B B' -> Isomorphism (A -> B) (A' -> B').
-Proof.
-  intros i1 i2.
-  exact (@Isomorphism_dep_fn A A' (fun _ => B) (fun _ => B') i1 (fun _ _ _ => i2)).
-Defined.
-
-Lemma Isomorphism_pair {A A' B B' : Type} :
-  Isomorphism A A' -> Isomorphism B B' -> Isomorphism (A * B) (A' * B').
-Proof.
-  intros [f1 t1 ft1 tf1] [f2 t2 ft2 tf2].
-  econstructor.
-  instantiate (1:= ltac:(intros [a b]; split; auto)).
-  instantiate (1:= ltac:(intros [a b]; split; auto)).
-  all: intros; intuition.
-  rewrite ft1, ft2; auto.
-  rewrite tf1, tf2; auto.
-Defined.
+Require Import VeriFFI.library.isomorphism.
+Require Import VeriFFI.library.meta.
 
 Ltac eq_refl_match :=
   match goal with
@@ -104,8 +23,6 @@ Ltac props x :=
   unfold id, eq_rect in *;
   clear P.
 
-Require Import VeriFFI.library.meta.
-
 (* opaque and transparent *)
 Inductive annotated : Type :=
 | TYPEPARAM : (forall (A : Type) `{Rep A}, annotated) -> annotated
@@ -114,8 +31,6 @@ Inductive annotated : Type :=
                     (option (prim_type -> annotated)) ->
                     annotated
 | TRANSPARENT : forall (A : Type) `{Rep A}, (option (A -> annotated)) -> annotated.
-
-Definition Rep_Z : Rep Z. Admitted.
 
 Theorem Rep_any : forall {A : Type}, Rep A. Admitted.
 
@@ -176,6 +91,13 @@ Defined.
 Definition model_spec (ep : extern_properties) : Prop :=
   model_spec_aux (type_desc ep) (prim_fn ep) (model_fn ep).
 
+Require Import VeriFFI.generator.all.
+
+Obligation Tactic := gen.
+MetaCoq Run (gen_for Z).
+MetaCoq Run (gen_for nat).
+MetaCoq Run (gen_for bool).
+
 Module IntVerification.
 
 Module Type UInt63.
@@ -230,8 +152,6 @@ Module C : UInt63.
 End C.
 
 Module UInt63_Proofs.
-
-  Definition Rep_Z : Rep Z. Admitted.
   Axiom Isomorphism_t : Isomorphism C.t FM.t.
 
   Definition from_Z_ep : extern_properties :=
@@ -419,8 +339,7 @@ Module Array_Proofs.
   Module FM := FM E.
   Module C := C E.
 
-  Definition Rep_nat : Rep nat. Admitted.
-  Definition Rep_t : Rep E.t. Admitted.
+  Definition Rep_t : Rep E.t := Rep_bool.
 
   Axiom Isomorphism_state : Isomorphism C.state FM.state.
 
@@ -516,12 +435,9 @@ Module Array_Proofs.
     props get_properties.
     prim_rewrites.
 
-    unfold fst at 2.
-
-    (* unfold FM.get, FM.set in *. *)
     eapply canon.nth_error_replace_nth.
     apply nth_error_repeat.
-    lia.
+    auto.
   Qed.
 
 End Array_Proofs.
