generator/Rep.v
@@ -12,7 +12,6 @@ Require Import ExtLib.Structures.Monads
 Require Import VeriFFI.generator.gen_utils.
 Require Import VeriFFI.library.base_representation.
 Require Import VeriFFI.library.meta.
-Require Import VeriFFI.generator.InGraph.
 
 (* Warning: MetaCoq doesn't use the Monad notation from ExtLib,
   therefore don't expect ExtLib functions to work with TemplateMonad. *)
@@ -23,12 +22,12 @@ Unset Strict Unquote Universe Mode.
 Ltac destruct_conj H :=
   match type of H with
   | @ex _ _ =>
-    let p := fresh "p" in
-    let m := fresh "M" in
+    let p := fresh "_p" in
+    let m := fresh "_M" in
     destruct H as [p m]; destruct_conj m
   | @and _ _ =>
-    let m1 := fresh "M" in
-    let m2 := fresh "M" in
+    let m1 := fresh "_M" in
+    let m2 := fresh "_M" in
     destruct H as [m1 m2]; destruct_conj m2
   | _ => idtac
   end.
@@ -57,7 +56,7 @@ Axiom graph_cRep_add_node : forall g to lb e p ts ps,
    -> graph_cRep (add_node g to lb e) p ts ps.
 
 Ltac mon n :=
-  let i := fresh "i" in
+  let i := fresh "_i" in
   match goal with
   | [|- @is_in_graph _ _ _ n _] =>
     let t := type of n in
@@ -80,6 +79,8 @@ Ltac prove_monotone :=
   induction x;
   unshelve (match goal with
   | [|- forall _ _, @is_in_graph _ _ _ ?this _] =>
+    let p := fresh "p" in
+    let H := fresh "H" in
     intros p H;
     hnf in H;
     destruct_conj H;
@@ -90,21 +91,144 @@ Ltac prove_monotone :=
     try (eauto || (eapply graph_cRep_add_node; eauto))
   end); auto.
 
-Ltac rep_gen :=
+Ltac rep_gen_tac :=
   intros;
   repeat (match goal with
           | [R : Rep _ |- _] => destruct R
           end);
   econstructor; [prove_has_v | prove_monotone].
 
+From MetaCoq.Template Require Import BasicAst.
+Require Import MetaCoq.Template.All.
+
+(* Warning: MetaCoq doesn't use the Monad notation from ExtLib,
+  therefore don't expect ExtLib functions to work with TemplateMonad. *)
+Import monad_utils.MCMonadNotation
+       ListNotations
+       MetaCoqNotations.
+
+Require Import VeriFFI.generator.InGraph.
+
+Definition generate_Rep_instance_type
+           (ind : inductive)
+           (mut : mutual_inductive_body)
+           (one : one_inductive_body) : TemplateMonad named_term :=
+  generate_instance_type ind mut one
+    (fun ty_name t =>
+      let n := "Rep_" ++ ty_name in
+      tProd (mkBindAnn (nNamed n) Relevant) (tApp <% Rep %> [tVar ty_name]) t)
+    (fun t => apply_to_pi_base (fun t' => tApp <% Rep %> [t']) t).
+
+(* Constructs the instance type for the type at hand,
+   checks if there's an instance for it. *)
+Definition find_missing_instance
+           (ind : inductive)
+           (mut : mutual_inductive_body)
+           (one : one_inductive_body) : TemplateMonad bool :=
+  tmMsg! ("Missing: " ++ string_of_inductive ind) ;;
+  generate_Rep_instance_type ind mut one >>=
+  DB.deBruijn >>= tmUnquoteTyped Type >>= has_instance.
+
+(* Take in a [global_declarations], which is a list of declarations,
+   and find the inductive declarations in that list
+   that do not have [InGraph] instances. *)
+Fixpoint find_missing_instances
+        (env : global_declarations) : TemplateMonad (list kername) :=
+    match env with
+    | (kn, InductiveDecl mut) :: env' =>
+      rest <- find_missing_instances env' ;;
+      ones <- monad_map_i
+                (fun i => find_missing_instance
+                            {| inductive_mind := kn ; inductive_ind := i |} mut)
+                (ind_bodies mut) ;;
+      if (fold_left andb ones true) (* if there are instances for all *)
+        then ret rest (* then this one is not missing *)
+        else ret (kn :: rest)
+    | _ :: env' => find_missing_instances env'
+    | nil =>
+      tmMsg "End of missings" ;;
+      ret nil
+    end.
+
+Definition add_instances_aux (kn : kername)
+                   (mut : mutual_inductive_body)
+                   (singles_tys : list (aname * named_term))
+                   (singles: list (def named_term)) : TemplateMonad _ :=
+  monad_map_i
+    (fun i one =>
+       let ind := {| inductive_mind := kn ; inductive_ind := i |} in
+       quantified <- quantified ind mut one "Rep_" <% Rep %> ;;
+       (* Now what can we do with this? *)
+       (*    Let's start by going to its named representation. *)
+       (* The reified type of the fully applied type constructor, *)
+       (*    but with free variables! *)
+       let tau := strip_quantifiers quantified in
+       let quantifiers : list (aname * named_term) :=
+           get_quantifiers id quantified in
+       extra_quantified <- DB.deBruijn (build_quantifiers tProd quantifiers
+                                                          (tApp <% Rep %> [tau])) ;;
+       instance_ty <- tmUnquoteTyped Type extra_quantified ;;
+       (* tmPrint prog';; *)
+       (* tmMsg "Inst" ;; *)
+       (* tmPrint instance ;; *)
+       (* Remove [tmEval] when MetaCoq issue 455 is fixed: *)
+       (* https://github.com/MetaCoq/metacoq/issues/455 *)
+       name <- tmFreshName =<< tmEval all ("Rep_" ++ ind_name one)%bs ;;
+       tmLemma name instance_ty ;;
+
+       (* (* This is sort of a hack. I couldn't use [tmUnquoteTyped] above *)
+       (*    because of a mysterious type error. (Coq's type errors in monadic *)
+       (*    contexts are just wild.) Therefore I had to [tmUnquote] it to get *)
+       (*    a Σ-type. But when you project the second field out of that, *)
+       (*    the type doesn't get evaluated to [InGraph _], it stays as *)
+       (*    [my_projT2 {| ... |}]. The same thing goes for the first projection, *)
+       (*    which is the type of the second projection. When the user prints *)
+       (*    their [InGraph] instance, Coq shows the unevaluated version. *)
+       (*    But we don't want to evaluate it [all] the way, that would unfoldd *)
+       (*    the references to other instances of [InGraph]. We only want to get *)
+       (*    the head normal form with [hnf]. *)
+       (*    We have to do this both for the instance body and its type. *) *)
+       (* tmEval hnf (my_projT2 instance) >>= *)
+       (*   tmDefinitionRed_ false name (Some hnf) ;; *)
+
+       (* Declare the new definition a type class instance *)
+       mp <- tmCurrentModPath tt ;;
+       tmExistingInstance (ConstRef (mp, name)) ;;
+
+       let fake_kn := (fst kn, ind_name one) in
+       tmMsg! ("Added Rep instance for " ++ string_of_kername fake_kn) ;;
+       ret tt) (ind_bodies mut).
+
+Definition add_instances (kn : kername) : TemplateMonad unit :=
+  mut <- tmQuoteInductive kn ;;
+  singles_tys <- singles_tys kn mut ;;
+  (* tmEval all singles_tys >>= tmPrint ;; *)
+  singles <- singles kn mut singles_tys ;;
+  (* tmEval all singles >>= tmPrint ;; *)
+  add_instances_aux kn mut singles_tys singles ;;
+  ret tt.
+
+(* Derives a [Rep] instance for the type constructor [Tau],
+   and the types its definition depends on. *)
+Definition rep_gen {kind : Type} (Tau : kind) : TemplateMonad unit :=
+  '(env, tau) <- tmQuoteRec Tau ;;
+  missing <- find_missing_instances (declarations env) ;;
+  monad_iter add_instances (rev missing).
+
+Obligation Tactic := rep_gen_tac.
+
+(* MetaCoq Run (in_graph_gen nat). *)
+(* MetaCoq Run (rep_gen nat). *)
+
 (* MetaCoq Run (in_graph_gen list). *)
 (* Instance Rep_list : forall A `{Rep_A: Rep A}, Rep (list A). *)
-(*   rep_gen. *)
+(*   (* intros. destruct Rep_A. *) *)
+(*   rep_gen_tac. *)
 (* Defined. *)
 
 (* MetaCoq Run (in_graph_gen nat). *)
 (* Instance Rep_nat : Rep nat. *)
-(*   rep_gen. *)
+(*   rep_gen_tac. *)
 (* Defined. *)
 
 (* MetaCoq Run (in_graph_gen bool). *)
