generator/all.v
@@ -1,0 +1,21 @@
+Require Import VeriFFI.library.base_representation.
+Require Import VeriFFI.library.meta.
+Require Import VeriFFI.generator.InGraph.
+Require Import VeriFFI.generator.Rep.
+Require Import VeriFFI.generator.Desc.
+
+From MetaCoq.Template Require Import BasicAst.
+Require Import MetaCoq.Template.All.
+
+(* Warning: MetaCoq doesn't use the Monad notation from ExtLib,
+  therefore don't expect ExtLib functions to work with TemplateMonad. *)
+Import monad_utils.MCMonadNotation.
+
+Definition gen_for {kind : Type} (Tau : kind) : TemplateMonad unit :=
+  @in_graph_gen kind Tau ;;
+  @rep_gen kind Tau.
+
+Definition desc_gen {T : Type} (ctor_val : T) : TemplateMonad unit :=
+  @Desc.desc_gen T ctor_val.
+
+Ltac gen := (try rep_gen_tac) || (try reconstructing).
